Fix the agree RA for entry nargs and finish fixing the CMDC adequacy

theories/rules/rules_base.v
@@ -6,21 +6,21 @@ From cap_machine Require Export cap_lang iris_extra stdpp_extra.
 From iris.algebra Require Import frac gmap.
 
 
-Definition entryUR : ucmra :=
-  (gmapUR Word (agreeR (leibnizO nat))).
+Definition entryR : cmra :=
+  (agreeR (leibnizO nat)).
 
 Class entryGpreS Σ := EntryGpreS {
   entryPreG_invPreG : invGpreS Σ;
-  entryPreG_rel :: inG Σ entryUR;
+  entryPreG_rel :: inG Σ entryR;
 }.
 
 Class entryGS Σ := EntryGS {
-  entryG_rel :: inG Σ entryUR;
-  γentry : gname
+  entryG_rel :: inG Σ entryR;
+  γentry : Word -> gname
 }.
 
 Definition entryPreΣ :=
-  #[ GFunctor entryUR ].
+  #[ GFunctor entryR ].
 
 Instance subG_entryPreΣ {Σ} :
   subG entryPreΣ Σ →
@@ -32,7 +32,7 @@ Section ENTRY_defs.
   Context {Σ:gFunctors} {entryg : entryGS Σ}.
 
   Definition ENTRY_def (w : Word) (n : nat) : iProp Σ :=
-    own γentry {[ w := to_agree n ]}.
+    own (γentry w) (to_agree n).
   Definition ENTRY_aux : { x | x = @ENTRY_def }. by eexists. Qed.
   Definition ENTRY := proj1_sig ENTRY_aux.
   Definition ENTRY_eq : @ENTRY = @ENTRY_def := proj2_sig ENTRY_aux.
@@ -45,14 +45,13 @@ Section ENTRY_defs.
     rewrite ENTRY_eq /ENTRY_def.
     iCombine "H1 H2" as "H".
     iDestruct (own_valid with "H") as "%".
-    apply singleton_valid, to_agree_op_inv in H.
+    apply to_agree_op_inv in H.
     done.
   Qed.
   Global Instance persistent_entry w n : Persistent (w ↦□ₑ n)%I.
   Proof.
     rewrite ENTRY_eq /ENTRY_def.
-    apply own_core_persistent.
-    apply gmap_core_id', agree_core_id.
+    apply _.
   Defined.
 
 
@@ -64,37 +63,34 @@ Section entryPre.
 
 
   Lemma entry_rel_init (m : gmap Word nat) :
-    ⊢ |==> (∃ γentry, own γentry ((to_agree <$> m) : entryUR)).
+    ⊢ |==> (∃ γentry, ([∗ map] w↦n ∈ m, own (γentry w) (to_agree n))).
   Proof.
-    iMod (own_alloc (A:= (entryUR)) (to_agree <$> m : entryUR)) as (γentry) "Hm".
-    { intros w.
-      destruct ((to_agree <$> m) !! w) eqn:Heq; rewrite Heq ; last done.
-      rewrite lookup_fmap_Some in Heq.
-      destruct Heq as (? & <- & ?).
-      done.
-    }
-    by iFrame.
+
+    induction m using map_ind.
+    - iModIntro.
+      iExists ( λ w, encode w).
+      by iApply big_sepM_empty.
+    - iMod IHm as (γentry) "IH".
+      iMod (own_alloc (A:= entryR) (to_agree x)) as (γx) "Hrel" ; first done.
+      iModIntro.
+      iExists (λ w, if (bool_decide (w = i)) then γx else γentry w).
+      iApply (big_sepM_insert with "[IH Hrel]");auto.
+      rewrite bool_decide_eq_true_2; auto; iFrame.
+      iApply (big_sepM_mono with "IH").
+      iIntros (k n Hk) "H".
+      rewrite bool_decide_eq_false_2; [done|].
+      by intros ->; rewrite H in Hk.
   Qed.
 
   Lemma entry_init m :
-    ⊢ |==> ∃ (entryg: entryGS Σ), own γentry ((to_agree <$> m) : entryUR).
+    ⊢ |==> ∃ (entryg: entryGS Σ), ([∗ map] w↦n ∈ m, w ↦□ₑ n).
   Proof.
     iMod entry_rel_init as (γ) "H".
     iExists (EntryGS _ _ _).
-    done.
+    by rewrite ENTRY_eq /ENTRY_def.
   Qed.
+
 End entryPre.
-
-
-(* Notation "w ↦ₑ{ q } n" := (pointsto (L:=Word) (V:=nat) w q n) *)
-(*   (at level 20, q at level 50, format "w  ↦ₑ{ q }  n") : bi_scope. *)
-(* Notation "w ↦ₑ n" := (pointsto (L:=Word) (V:=nat) w (DfracOwn 1) n) (at level 20) : bi_scope. *)
-(* Notation "w ↦□ₑ n" := (pointsto (L:=Word) (V:=nat) w DfracDiscarded n) (at level 20) : bi_scope. *)
-
-(* Class entryG Σ := *)
-(*   EntryG { entry_genG :: gen_heapGS Word nat Σ; (* entry points argument *) }. *)
-
-
 
 (* CMRA for Cerise *)
 Class ceriseG Σ :=
